src/3d/Simplify.fst
@@ -59,8 +59,11 @@ and simplify_typ (env:T.env_t) (t:typ)
     | Pointer t -> {t with v=Pointer (simplify_typ env t)}
     | Type_app s b ps ->
       let ps = List.map (simplify_typ_param env) ps in
-      let s = B.resolve_typedef_abbrev (fst env) s in
-      { t with v = Type_app s b ps }
+      let s = B.resolve_record_case_outputtype_name (fst env) s in
+      let t = { t with v = Type_app s b ps } in
+      if Options.get_interpret()
+      then B.unfold_typ_abbrev_only (fst env) t
+      else t
 
 and simplify_out_expr_node (env:T.env_t) (oe:with_meta_t out_expr')
   : ML (with_meta_t out_expr')
